Add a number of theories

theories/Logic.v
@@ -1,37 +1,67 @@
-Require Import Hoare.State.
+Require Export Hoare.State.
 
-Declare Scope hoare_logic_scope.
-Open Scope hoare_logic_scope.
+From Coq Require Import Classes.EquivDec.
 
 Section logic.
-  Generalizable All Variables.
+  Generalizable Variables Σ.
 
-  Context (T U : Type).
-  
+  Context {T U : Type}.
   Implicit Type s : state T U.
 
-  Definition Assertion := state T U -> Prop.
+  Class Expression (A : Type) {V} := exp_R (exp : A) (s : state T U) (v : V) : Prop.
+  Class Statement (A : Type) := stm_R (stm : A) (s s' : state T U) : Prop.
 
+  Definition Assertion := state T U -> Prop.
   Definition assert_implies (P Q : Assertion) : Prop :=
     forall s, P s -> Q s.
-  Notation "P ⇾ Q" := (assert_implies P Q) (at level 80) : hoare_logic_scope.
-
   Definition assert_iff (P Q : Assertion) : Prop :=
     forall s, P s -> Q s /\ Q s -> P s.
-  Notation "P ⇿ Q" := (assert_iff P Q) (at level 80) : hoare_logic_scope.
-
-  Class Statement (A : Type) := {
-    stm_R (stm : A) s s' : Prop
-  }.
-  Notation "⟨ x , y ⟩ ⇒ z" := (stm_R x y z)
-    (at level 40, y at level 99, x constr at level 99, z constr at level 98).
-
+  Definition assert_and (P Q : Assertion) : Assertion :=
+    fun s => P s /\ Q s.
   Definition hoare_triple `{Statement Σ} (P : Assertion) (stm : Σ) (Q : Assertion) : Prop :=
-    forall s s', ⟨stm, s⟩ ⇒ s' -> P s -> Q s'.
-  Notation "{{ P }} s {{ Q }}" := (hoare_triple P s Q)
-    (at level 90, s at level 99) : hoare_logic_scope.
-
-  Theorem hoare_post_tauto `{Statement Σ} :
-    forall (P Q : Assertion) (stm : Σ), (forall s, Q s) -> {{ P }} stm {{ Q }}.
-  Proof. unfold hoare_triple. intros. apply H0. Qed.
+    forall s s', stm_R stm s s' -> P s -> Q s'.
+  Definition assert_sub `{EqDec T} `{Expression Σ U} (x : T) (exp : Σ) (P : Assertion) : Assertion :=
+    fun s => forall n, exp_R exp s n -> P (x ↦ n ; s).
 End logic.
+
+Global Hint Unfold assert_implies hoare_triple assert_sub : core.
+
+Declare Scope hoare_logic_scope.
+Declare Custom Entry lang.
+
+Notation "P [ x ↦ a ]" := (assert_sub x a P)
+  (at level 10, x at next level) : hoare_logic_scope.
+Notation "⟦ exp ⟧ s ⇒ r" := (exp_R exp s r)
+  (at level 40,
+    exp custom lang at level 99,
+    s constr at level 99,
+    r constr at level 98).
+Notation "P ⇾ Q" := (assert_implies P Q) (at level 80) : hoare_logic_scope.
+Notation "P ⇿ Q" := (assert_iff P Q) (at level 80) : hoare_logic_scope.
+Notation "⟨ stm , s ⟩ ⇒ s'" := (stm_R stm s s')
+    (at level 40, s at level 99,
+      stm custom lang at level 99,
+      s' constr at level 98).
+Notation "{{ P }} stm {{ Q }}" := (hoare_triple P stm Q)
+    (at level 90, stm custom lang at level 99) : hoare_logic_scope.
+Notation "<{ e }>" := e (at level 0, e custom lang at level 99) : hoare_logic_scope.
+Notation "( e )" := e (in custom lang, e at level 99) : hoare_logic_scope.
+Notation "e" := e (in custom lang at level 0, e constr at level 0) : hoare_logic_scope.
+
+Section lemmas.
+  Generalizable Variables Σ.
+  Context {T U : Type} (P P' Q Q' : @Assertion T U).
+  Open Scope hoare_logic_scope.
+
+  Lemma hoare_imp_pre `{@Statement T U Σ} (stm : Σ) :
+    {{ P' }} stm {{ Q }} -> P ⇾ P' -> {{ P }} stm {{ Q }}.
+  Proof. eauto. Qed.
+
+  Lemma hoare_imp_post `{@Statement T U Σ} (stm : Σ) :
+    {{ P }} stm {{ Q }} -> Q ⇾ Q' -> {{ P }} stm {{ Q' }}.
+  Proof. eauto. Qed.
+
+  Lemma hoare_imp_assert `{@Statement T U Σ} (stm : Σ) :
+    {{ P' }} stm {{ Q }} -> P ⇾ P' -> Q ⇾ Q' -> {{ P }} stm {{ Q' }}.
+  Proof. eauto. Qed.
+End lemmas.
