theories/While.v
@@ -1,49 +1,18 @@
-(** This file defines the syntax and semantics for the "While"
-deeply embedded language. It is based on [1].
-
-[1]: Hanne Riis Nielson, Flemming Nielson: Semantics with applications - a
-     formal introduction. Wiley professional computing, Wiley 1992,
-     ISBN 978-0-471-92980-2, pp. I-XII, 1-240 
-
-This was mostly copied from:
-
-https://softwarefoundations.cis.upenn.edu/lf-current/Imp.html *)
+(** This file defines the syntax and semantics for the "Stack" language. *)
 
 Set Warnings "-notation-overridden".
 
+Require Import Hoare.Logic.
 Require Import Hoare.State.
 
-From Coq Require Import Arith.Arith.
-From Coq Require Import Bool.Bool.
-From Coq Require Import Classes.EquivDec.
-From Coq Require Import Strings.String.
+From Coq Require Export Arith.Arith.
+From Coq Require Export Bool.Bool.
+From Coq Require Export Classes.EquivDec.
+From Coq Require Export Strings.String.
 
-Declare Custom Entry stm.
-Declare Scope stm_scope.
+Open Scope hoare_logic_scope.
 
-Open Scope stm_scope.
-
-Notation "<{ e }>" := e (at level 0, e custom stm at level 99) : stm_scope.
-Notation "( e )" := e (in custom stm, e at level 99) : stm_scope.
-Notation "e" := e (in custom stm at level 0, e constr at level 0) : stm_scope.
-
-Reserved Notation "⟨ x , y ⟩ ⇒ z"
-  (at level 40, y custom stm at level 99, x constr at level 99, z constr at level 98).
-
-#[universes(template)]
-Class Evaluable (T S U : Type) :=
-  {
-    eval_R : T -> S -> U -> Prop
-  }.
-Notation "⟦ t ⟧ s ⇒ u" := (eval_R t s u)
-  (at level 40,
-    t custom stm at level 99,
-    s constr at level 99,
-    u constr at level 98).
-
-(** State as used in the "While" language. *)
 Local Instance string_eq_eqdec : EqDec string eq := string_dec.
-Definition while_state := state string nat.
 
 Inductive aexp :=
   | ANum : nat -> aexp (* numeral: n *)
@@ -53,36 +22,28 @@ Inductive aexp :=
   | AMin : aexp -> aexp -> aexp. (* subtraction: a1 - a2 *)
 Coercion AVar : string >-> aexp.
 Coercion ANum : nat >-> aexp.
-Infix "+" := AAdd (in custom stm at level 50, left associativity).
-Infix "*" := AMult (in custom stm at level 40, left associativity).
-Infix "-" := AMin (in custom stm at level 50, left associativity).
-Inductive aexp_R : aexp -> while_state -> nat -> Prop :=
-  | ANum_R (s : while_state) (n : nat) : 
-    (*────────────*)
+Infix "+" := AAdd (in custom lang at level 50, left associativity).
+Infix "*" := AMult (in custom lang at level 40, left associativity).
+Infix "-" := AMin (in custom lang at level 50, left associativity).
+Inductive aexp_R : aexp -> state string nat -> nat -> Prop :=
+  | ANum_R s (n : nat) :
       aexp_R n s n
-  | AVar_R (s : while_state) (x : string) (n : nat) :
+  | AVar_R s x n :
       s x = Some n ->
-    (*───────────────*)
-        aexp_R x s n
-  | AAdd_R (s : while_state) (a1 a2 : aexp) (n1 n2 : nat) :
-             aexp_R a1 s n1 ->
-             aexp_R a2 s n2 ->
-    (*──────────────────────────────*)
+      aexp_R x s n
+  | AAdd_R s a1 a2 n1 n2 :
+      aexp_R a1 s n1 ->
+      aexp_R a2 s n2 ->
       aexp_R <{a1 + a2}> s (n1 + n2)
-  | AMult_R (s : while_state) (a1 a2 : aexp) (n1 n2 : nat) :
-             aexp_R a1 s n1 ->
-             aexp_R a2 s n2 ->
-    (*──────────────────────────────*)
+  | AMult_R s a1 a2 n1 n2 :
+      aexp_R a1 s n1 ->
+      aexp_R a2 s n2 ->
       aexp_R <{a1 * a2}> s (n1 * n2)
-  | AMin_R (s : while_state) (a1 a2 : aexp) (n1 n2 : nat) :
-             aexp_R a1 s n1 ->
-             aexp_R a2 s n2 ->
-    (*──────────────────────────────*)
+  | AMin_R s a1 a2 n1 n2 :
+      aexp_R a1 s n1 ->
+      aexp_R a2 s n2 ->
       aexp_R <{a1 - a2}> s (n1 - n2).
-Local Instance aexp_Evaluable : Evaluable aexp while_state nat :=
-  {
-    eval_R := aexp_R
-  }.
+Global Instance aexp_Expression : Expression aexp := aexp_R.
 
 Inductive bexp :=
   | BTrue : bexp (* true *)
@@ -91,42 +52,33 @@ Inductive bexp :=
   | BLeq : aexp -> aexp -> bexp (* less-than-or-equals: a1 ≤ a2 *)
   | BNeg : bexp -> bexp (* negation: ¬b *)
   | BAnd : bexp -> bexp -> bexp. (* conjunction: b1 ∧ b2 *)
-Notation "'true'" := BTrue (in custom stm at level 0).
-Notation "'false'" := BFalse (in custom stm at level 0).
-Infix "=" := BEq (in custom stm at level 70, no associativity).
-Infix "≤" := BLeq (in custom stm at level 70, no associativity).
-Notation "¬ b" := (BNeg b) (in custom stm at level 75, right associativity).
-Infix "∧" := BAnd (in custom stm at level 80, left associativity).
-Inductive bexp_R : bexp -> while_state -> bool -> Prop :=
-  | BTrue_R (s : while_state) :
-    (*────────────────────────*)
-      bexp_R (<{true}>) s true
-  | BFalse_R (s : while_state) :
-    (*──────────────────────────*)
-      bexp_R (<{false}>) s false
-  | BEq_R (s : while_state) (a1 a2 : aexp) (n1 n2 : nat) :
-               ⟦a1⟧s ⇒ n1 ->
-               ⟦a2⟧s ⇒ n2 ->
-    (*─────────────────────────────────*)
+Notation "'true'" := BTrue (in custom lang at level 0).
+Notation "'false'" := BFalse (in custom lang at level 0).
+Infix "=" := BEq (in custom lang at level 70, no associativity).
+Infix "<=" := BLeq (in custom lang at level 70, no associativity).
+Notation "! b" := (BNeg b) (in custom lang at level 75, right associativity).
+Infix "&&" := BAnd (in custom lang at level 80, left associativity).
+Inductive bexp_R : bexp -> state string nat -> bool -> Prop :=
+  | BTrue_R s :
+      bexp_R <{true}> s true
+  | BFalse_R s :
+      bexp_R <{false}> s false
+  | BEq_R s a1 a2 n1 n2 :
+      ⟦a1⟧s ⇒ n1 ->
+      ⟦a2⟧s ⇒ n2 ->
       bexp_R (<{a1 = a2}>) s (n1 =? n2)
-  | BLeq_R (s : while_state) (a1 a2 : aexp) (n1 n2 : nat) :
-                ⟦a1⟧s ⇒ n1 ->
-                ⟦a2⟧s ⇒ n2 ->
-    (*──────────────────────────────────*)
-      bexp_R (<{a1 ≤ a2}>) s (n1 <=? n2)
-  | BNeg_R (s : while_state) (b : bexp) (b' : bool) :
-            bexp_R b s b' ->
-    (*───────────────────────────*)
-      bexp_R (<{¬b}>) s (negb b')
-  | BAnd_R (s : while_state) (b1 b2 : bexp) (b1' b2' : bool) :
-                bexp_R b1 s b1' ->
-                bexp_R b2 s b2' ->
-    (*─────────────────────────────────────*)
-      bexp_R (<{b1 ∧ b2}>) s (andb b1' b2').
-Local Instance bexp_Evaluable : Evaluable bexp while_state bool :=
-  {
-    eval_R := bexp_R
-  }.
+  | BLeq_R s a1 a2 n1 n2 :
+      ⟦a1⟧s ⇒ n1 ->
+      ⟦a2⟧s ⇒ n2 ->
+      bexp_R <{a1 <= a2}> s (n1 <=? n2)
+  | BNeg_R s b b' :
+      bexp_R b s b' ->
+      bexp_R (<{!b}>) s (negb b')
+  | BAnd_R s b1 b2 b1' b2' :
+      bexp_R b1 s b1' ->
+      bexp_R b2 s b2' ->
+      bexp_R (<{b1 && b2}>) s (andb b1' b2').
+Global Instance bexp_Expression : Expression bexp := bexp_R.
 
 Inductive stm :=
   | SAsgn : string -> aexp -> stm (* assignment: x := a *)
@@ -134,51 +86,57 @@ Inductive stm :=
   | SSeq : stm -> stm -> stm (* sequence: s1 ; s2 *)
   | SIf : bexp -> stm -> stm -> stm (* conditional: if b then s1 else s2 end *)
   | SWhile : bexp -> stm -> stm. (* looping: while b do s end *)
-Notation "'skip'" := SSkip (in custom stm at level 0) : stm_scope.
+Notation "'skip'" := SSkip (in custom lang at level 0) : hoare_logic_scope.
 Notation "x := a" := (SAsgn x a)
-  (in custom stm at level 0, x constr at level 0, a at level 85, no associativity) : stm_scope.
+  (in custom lang at level 0, x constr at level 0, a at level 85, no associativity) : hoare_logic_scope.
 Notation "s1 ; s2" := (SSeq s1 s2)
-  (in custom stm at level 90, right associativity) : stm_scope.
+  (in custom lang at level 90, right associativity) : hoare_logic_scope.
 Notation "'if' b 'then' s1 'else' s2 'end'" := (SIf b s1 s2)
-  (in custom stm at level 89, b at level 99, s1 at level 99, s1 at level 99) : stm_scope.
+  (in custom lang at level 89, b at level 99, s1 at level 99, s1 at level 99) : hoare_logic_scope.
 Notation "'while' b 'do' s 'end'" := (SWhile b s)
-  (in custom stm at level 89, b at level 99, s at level 99) : stm_scope.
-
-Reserved Notation "⟨ x , y ⟩ ⇒ z"
-  (at level 40, y custom stm at level 99, x constr at level 99, z constr at level 98).
-
-(** Operational semantics of "While" *)
-Inductive stm_R : stm -> while_state -> while_state -> Prop :=
+  (in custom lang at level 89, b at level 99, s at level 99) : hoare_logic_scope.
+Inductive stm_R : stm -> state string nat -> state string nat -> Prop :=
   | SAsgn_R s x a n :
-               ⟦a⟧s ⇒ n ->
-    (*───────────────────────────────*)
-      ⟨<{x := a}>, s⟩ ⇒ (x ↦ n ; s)
+      ⟦a⟧s ⇒ n ->
+      stm_R <{x := a}> s (x ↦ n ; s)
   | SSkip_R s :
-    (*─────────────────*)
-      ⟨<{skip}>, s⟩ ⇒ s
+      stm_R <{skip}> s s
   | SSeq_R s s' s'' S1 S2 :
-       ⟨<{S1}>, s⟩ ⇒ s' ->
-      ⟨<{S2}>, s'⟩ ⇒ s'' ->
-    (*──────────────────────*)
-      ⟨<{S1; S2}>, s⟩ ⇒ s''
+      stm_R <{S1}> s s' ->
+      stm_R <{S2}> s' s'' ->
+      stm_R <{S1; S2}> s s''
   | SIf_R_True s s' b S1 S2 :
-                  ⟦b⟧s ⇒ true ->
-               ⟨<{S1}>, s⟩ ⇒ s' ->
-    (*───────────────────────────────────────*)
-      ⟨<{if b then S1 else S2 end}>, s⟩ ⇒ s'
+      ⟦b⟧s ⇒ true ->
+      stm_R <{S1}> s s' ->
+      stm_R <{if b then S1 else S2 end}> s s'
   | SIf_R_False s s' b S1 S2 :
-                  ⟦b⟧s ⇒ false ->
-               ⟨<{S2}>, s⟩ ⇒ s' ->
-    (*───────────────────────────────────────*)
-      ⟨<{if b then S1 else S2 end}>, s⟩ ⇒ s'
+      ⟦b⟧s ⇒ false ->
+      stm_R <{S2}> s s' ->
+      stm_R <{if b then S1 else S2 end}> s s'
   | SWhile_R_True s s' s'' b S :
-                 ⟦b⟧s ⇒ true ->
-               ⟨<{S}>, s⟩ ⇒ s' ->
-      ⟨<{while b do S end}>, s'⟩ ⇒ s'' ->
-    (*────────────────────────────────────*)
-         ⟨<{while b do S end}>, s⟩ ⇒ s''
+      ⟦b⟧s ⇒ true ->
+      stm_R <{S}> s s' ->
+      stm_R <{while b do S end}> s' s'' ->
+      stm_R <{while b do S end}> s s''
   | SWhile_R_False s b S :
-            ⟦b⟧s ⇒ false ->
-  (*──────────────────────────────*)
-    ⟨<{while b do S end}>, s⟩ ⇒ s
-where "⟨ stm , st ⟩ ⇒ st'" := (stm_R stm st st').
+      ⟦b⟧s ⇒ false ->
+      stm_R <{while b do S end}> s s.
+Global Instance stm_Statement : Statement stm := stm_R.
+
+Section rules.
+  Context (P Q : @Assertion string nat).
+
+  Lemma hoare_skip : {{ P }} skip {{ P }}.
+  Proof.
+    unfold hoare_triple. intros.
+    inversion H; subst; assumption.
+  Qed.
+
+  Lemma hoare_assn (a : aexp) x : {{ Q[x ↦ a] }} x := a {{ Q }}.
+  Proof.
+    unfold hoare_triple.
+    intros. inversion H. subst.
+    unfold assert_sub in H0. auto.
+  Qed.
+
+  
