theories/State.v
@@ -2,13 +2,17 @@
 
 Require Import Coq.Classes.EquivDec.
 
-Definition state (T U : Type) := T -> option U.
-Definition mod_state {T U} `{EqDec T}
-  (st : state T U) (x : T) (y : U) : state T U
-:= fun x' => if x == x' then Some y else st x'.
-Definition empty_state {T U} : state T U :=
-  fun _ => None.
+Section state.
+  Definition state T U := T -> option U.
+  Definition mod_state {T U} `{EqDec T}
+    (st : state T U) (x : T) (y : U) : state T U
+  := fun x' => if x == x' then Some y else st x'.
+  Definition empty_state {T U} : state T U :=
+    fun _ => None.
+End state.
 
 Notation "∅" := empty_state.
 Notation "x ↦ y ; st" := (mod_state st x y)
   (at level 100, y at next level, right associativity).
+Notation "x ↦ y" := (mod_state ∅ x y)
+  (at level 100, y at next level, no associativity).
